src/ProbabilisticProgramming/Loops.dfy
@@ -1,0 +1,228 @@
+/*******************************************************************************
+ *  Copyright by the contributors to the Dafny Project
+ *  SPDX-License-Identifier: MIT
+ *******************************************************************************/
+
+module Loops {
+  import Monad
+  import Quantifier
+  import Independence
+  import Random
+
+  /************
+   Definitions
+  ************/
+
+  // Definition 37
+  function WhileCut<A>(condition: A -> bool, body: A -> Monad.Hurd<A>, n: nat, init: A): Monad.Hurd<A> {
+    if n == 0 then
+      Monad.Return(init)
+    else (
+           if condition(init) then
+             Monad.Bind(body(init), (a: A) => WhileCut(condition, body, n-1, a))
+           else
+             Monad.Return(init)
+         )
+  }
+
+  // Definition 39 / True iff Prob(iset s | While(condition, body, a)(s) terminates) == 1
+  ghost predicate WhileTerminates<A(!new)>(condition: A -> bool, body: A -> Monad.Hurd<A>) {
+    var p := (a: A) =>
+               (s: Random.Bitstream) => exists n :: !condition(WhileCut(condition, body, n, a)(s).0);
+    forall a :: Quantifier.AlmostSurely(p(a))
+  }
+
+  // Theorem 38
+  function While<A>(condition: A -> bool, body: A -> Monad.Hurd<A>, init: A): (f: Monad.Hurd<A>)
+    requires WhileTerminates(condition, body)
+  {
+    assume {:axiom} false; // assume termination
+    if condition(init) then
+      Monad.Bind(body(init), (a': A) => While(condition, body, a'))
+    else
+      Monad.Return(init)
+  }
+
+  method WhileImperative<A>(condition: A -> bool, body: A -> Monad.Hurd<A>, init: A, s: Random.Bitstream) returns (t: (A, Random.Bitstream))
+    requires WhileTerminates(condition, body)
+    ensures While(condition, body, init)(s) == t
+    decreases *
+  {
+    while condition(init)
+      decreases *
+    {
+      var (a, s) := body(init)(s);
+    }
+    return (init, s);
+  }
+
+  method WhileImperativeAlternative<A>(condition: A -> bool, body: A -> Monad.Hurd<A>, init: A, s: Random.Bitstream) returns (t: (A, Random.Bitstream))
+    requires WhileTerminates(condition, body)
+    ensures While(condition, body, init)(s) == t
+    decreases *
+  {
+    while true
+      decreases *
+    {
+      if !condition(init) {
+        return (init, s);
+      } else {
+        var (a, s) := body(init)(s);
+      }
+    }
+  }
+
+  ghost predicate UntilTerminates<A(!new)>(proposal: Monad.Hurd<A>, accept: A -> bool) {
+    var reject := (a: A) => !accept(a);
+    var body := (a: A) => proposal;
+    WhileTerminates(reject, body)
+  }
+
+  // Definition 44
+  function Until<A>(proposal: Monad.Hurd<A>, accept: A -> bool): (f: Monad.Hurd<A>)
+    requires UntilTerminates(proposal, accept)
+    ensures
+      var reject := (a: A) => !accept(a);
+      var body := (a: A) => proposal;
+      forall s :: f(s) == While(reject, body, proposal(s).0)(proposal(s).1)
+  {
+    var reject := (a: A) => !accept(a);
+    var body := (a: A) => proposal;
+    Monad.Bind(proposal, (a: A) => While(reject, body, a))
+  }
+
+  method UntilImperative<A>(proposal: Monad.Hurd<A>, accept: A -> bool, s: Random.Bitstream) returns (t: (A, Random.Bitstream))
+    requires UntilTerminates(proposal, accept)
+    ensures t == Until(proposal, accept)(s)
+    decreases *
+  {
+    var reject := (a: A) => !accept(a);
+    var body := (a: A) => proposal;
+    t := WhileImperative(reject, body, proposal(s).0, proposal(s).1);
+  }
+
+  function WhileLoopExitsAfterOneIteration<A(!new)>(body: A -> Monad.Hurd<A>, condition: A -> bool, init: A): (Random.Bitstream -> bool) {
+    (s: Random.Bitstream) =>
+      !condition(body(init)(s).0)
+  }
+
+  function ProposalIsAccepted<A(!new)>(proposal: Monad.Hurd<A>, accept: A -> bool): (Random.Bitstream -> bool) {
+    (s: Random.Bitstream) =>
+      accept(proposal(s).0)
+  }
+
+  function UntilLoopResultIsAccepted<A>(proposal: Monad.Hurd<A>, accept: A -> bool): (Random.Bitstream -> bool)
+    requires UntilTerminates(proposal, accept)
+  {
+    (s: Random.Bitstream) =>
+      accept(Until(proposal, accept)(s).0)
+  }
+
+  ghost function UntilLoopResultHasProperty<A>(proposal: Monad.Hurd<A>, accept: A -> bool, property: A -> bool): iset<Random.Bitstream>
+    requires UntilTerminates(proposal, accept)
+  {
+    iset s | property(Until(proposal, accept)(s).0)
+  }
+
+  ghost function ProposalIsAcceptedAndHasProperty<A>(proposal: Monad.Hurd<A>, accept: A -> bool, property: A -> bool): iset<Random.Bitstream>
+  {
+    iset s | property(proposal(s).0) && accept(proposal(s).0)
+  }
+
+  ghost function ProposalAcceptedEvent<A>(proposal: Monad.Hurd<A>, accept: A -> bool): iset<Random.Bitstream>
+  {
+    iset s | accept(proposal(s).0)
+  }
+
+
+  /*******
+   Lemmas
+  *******/
+
+  lemma EnsureUntilTerminates<A(!new)>(proposal: Monad.Hurd<A>, accept: A -> bool)
+    requires Independence.IsIndep(proposal)
+    requires Quantifier.WithPosProb((s: Random.Bitstream) => accept(proposal(s).0))
+    ensures UntilTerminates(proposal, accept)
+  {
+    var reject := (a: A) => !accept(a);
+    var body := (a: A) => proposal;
+    var proposalIsAccepted := (s: Random.Bitstream) => accept(proposal(s).0);
+    assert UntilTerminates(proposal, accept) by {
+      forall a: A ensures Independence.IsIndep(body(a)) {
+        assert body(a) == proposal;
+      }
+      forall a: A ensures Quantifier.WithPosProb(WhileLoopExitsAfterOneIteration(body, reject, a)) {
+        assert Quantifier.WithPosProb(proposalIsAccepted);
+        assert (iset s | proposalIsAccepted(s)) == (iset s | WhileLoopExitsAfterOneIteration(body, reject, a)(s));
+      }
+      assert WhileTerminates(reject, body) by {
+        EnsureWhileTerminates(reject, body);
+      }
+    }
+  }
+
+  // (Equation 3.30) / Sufficient conditions for while-loop termination
+  lemma {:axiom} EnsureWhileTerminates<A(!new)>(condition: A -> bool, body: A -> Monad.Hurd<A>)
+    requires forall a :: Independence.IsIndep(body(a))
+    requires forall a :: Quantifier.WithPosProb(WhileLoopExitsAfterOneIteration(body, condition, a))
+    ensures WhileTerminates(condition, body)
+
+  // Theorem 45 (wrong!) / PROB_BERN_UNTIL (correct!)
+  lemma {:axiom} UntilProbabilityFraction<A>(proposal: Monad.Hurd<A>, accept: A -> bool, d: A -> bool)
+    requires Independence.IsIndep(proposal)
+    requires Quantifier.WithPosProb(ProposalIsAccepted(proposal, accept))
+    ensures UntilTerminates(proposal, accept)
+    ensures
+      && UntilLoopResultHasProperty(proposal, accept, d) in Random.eventSpace
+      && ProposalIsAcceptedAndHasProperty(proposal, accept, d) in Random.eventSpace
+      && ProposalAcceptedEvent(proposal, accept) in Random.eventSpace
+      && Random.Prob(ProposalAcceptedEvent(proposal, accept)) != 0.0
+      && Random.Prob(UntilLoopResultHasProperty(proposal, accept, d)) == Random.Prob(ProposalIsAcceptedAndHasProperty(proposal, accept, d)) / Random.Prob(ProposalAcceptedEvent(proposal, accept))
+
+  // Equation (3.39)
+  lemma {:axiom} UntilAsBind<A(!new)>(proposal: Monad.Hurd<A>, accept: A -> bool, s: Random.Bitstream)
+    requires Independence.IsIndep(proposal)
+    requires Quantifier.WithPosProb(ProposalIsAccepted(proposal, accept))
+    ensures UntilTerminates(proposal, accept)
+    ensures Until(proposal, accept) == Monad.Bind(proposal, (x: A) => if accept(x) then Monad.Return(x) else Until(proposal, accept))
+
+  // Equation (3.40)
+  lemma EnsureUntilTerminatesAndForAll<A(!new)>(proposal: Monad.Hurd<A>, accept: A -> bool)
+    requires Independence.IsIndep(proposal)
+    requires Quantifier.WithPosProb(ProposalIsAccepted(proposal, accept))
+    ensures UntilTerminates(proposal, accept)
+    ensures Quantifier.AlmostSurely(UntilLoopResultIsAccepted(proposal, accept))
+  {
+    EnsureUntilTerminates(proposal, accept);
+    assume {:axiom} Quantifier.AlmostSurely(UntilLoopResultIsAccepted(proposal, accept)); // add later
+  }
+
+  lemma WhileIsIndep<A(!new)>(condition: A -> bool, body: A -> Monad.Hurd<A>, init: A)
+    requires forall a: A :: Independence.IsIndep(body(a))
+    requires WhileTerminates(condition, body)
+    ensures Independence.IsIndep(While(condition, body, init))
+  {
+    if condition(init) {
+      forall a ensures Independence.IsIndep(While(condition, body, a)) {
+        assume {:axiom} false; // circular reasoning, rewrite this proof
+        WhileIsIndep(condition, body, a);
+      }
+      Independence.IndepFnIsCompositional(body(init), a => While(condition, body, a));
+    } else {
+      Independence.ReturnIsIndep(init);
+    }
+  }
+
+  lemma UntilIsIndep<A(!new)>(proposal: Monad.Hurd<A>, accept: A -> bool)
+    requires Independence.IsIndep(proposal)
+    requires UntilTerminates(proposal, accept)
+    ensures Independence.IsIndep(Until(proposal, accept))
+  {
+    var reject := (a: A) => !accept(a);
+    var body := (a: A) => proposal;
+    forall init: A {
+      WhileIsIndep(reject, body, init);
+    }
+    Independence.IndepFnIsCompositional(proposal, (init: A) => While(reject, body, init));
+  }
+}
