src/ProbabilisticProgramming/RandomSource.dfy
@@ -1,0 +1,27 @@
+/*******************************************************************************
+ *  Copyright by the contributors to the Dafny Project
+ *  SPDX-License-Identifier: MIT
+ *******************************************************************************/
+
+module Random {
+  import Measures
+
+  /************
+   Definitions
+  ************/
+
+  type Bitstream = nat -> bool
+
+  ghost const sampleSpace: iset<Bitstream> := iset s: Bitstream
+
+  ghost const eventSpace: iset<iset<Bitstream>>
+
+  ghost function Prob(event: iset<Bitstream>): real
+
+  /*******
+   Lemmas
+  *******/
+
+  lemma {:axiom} ProbIsProbabilityMeasure()
+    ensures Measures.IsProbability(eventSpace, sampleSpace, Prob)
+}
